modified the implementation to be similar to verify this challenge

main.dfy
@@ -1,237 +1,144 @@
-datatype State = IDLE | GAME_AVAILABLE | BET_PLACED | TRANSFERING
-
 datatype Coin = HEADS | TAILS
 
-trait Account{
+datatype State = IDLE | GAME_AVAILABLE | BET_PLACED
+
+datatype Msg = Msg(sender: Account, value: int) 
+
+
+trait Account {
   var balance: int
-  const isContract: bool
-}
+  var address: string
 
-class Sender extends Account{
-  var name: string
-
-  constructor()
-    ensures this.balance >= 0
-  {
-    this.name := "";
-    this.balance := 0;
-    this.isContract := false;
-  }
-
-  constructor FromName(name: string)
-    ensures this.balance >= 0
-  {
-    this.name := name;
-    this.balance := 0;
-    this.isContract := false;
-
-  }
-  constructor FromNameBalance(name: string, balance: int)
-    requires balance > 0
-    ensures this.balance == balance
-    ensures this.balance > 0
-  {
-    this.name := name;
-    this.balance := balance;
-    this.isContract := false;
-
-  }
-
-  method transfer(person: Sender, amount: int)
-    requires person != this
-    modifies this, person
-    requires this != person
+  method transfer(to: Account, amount: int)
+    requires to != this
     requires 0 < amount <= this.balance
-    requires person.balance >= 0
-    ensures this.balance ==  old(this.balance) - amount
-    ensures person.balance == old(person.balance) + amount
-    ensures old(person.balance) <= person.balance
-    ensures old(person.balance) <= person.balance + amount
-    ensures amount <= person.balance
-    ensures this.balance >= 0
-    ensures person.balance >= 0
+    requires to.balance >= 0
+    modifies this, to
+    ensures this.balance == old(this.balance) - amount
+    ensures to.balance == old(to.balance) + amount
   {
-
     this.balance := this.balance - amount;
-    person.balance := person.balance + amount;
+    to.balance := to.balance + amount;
   }
 }
 
-class Contract extends Account{
-  var name: string
-  var operator: Sender
-  var state: State
+class UserAccount extends Account {
+
+    constructor(initialBal: int) 
+        ensures balance == initialBal
+    {
+        balance := initialBal;
+    }
+}
+
+class Casino extends Account{
+  var operator: Account
+  var player: Account
+  var pot: int
+  var hashedNumber: int
   var guess: Coin
   var bet: int
-  var player: Sender
-  var hashedNumber: int
+  var state: State
 
-  function cryptohash(number: int) : (o:int)
+  function cryptohash(number: int): int
     ensures cryptohash(number) >= 0
-    ensures o == cryptohash(number)
   {
     if number < 0 then -(number * 31 + 17) else number * 31 + 17
   }
 
-  function getCoinFromGuess(guess: bool) : Coin{
-    if guess == true then TAILS
-    else HEADS
+  function getCoinFromNumber(number: int): Coin {
+    if number % 2 == 0 then HEADS else TAILS
   }
 
-
-  constructor(sender: Sender, guess: Coin)
-    ensures this.operator != this.player
+  constructor(msg: Msg)
+    ensures this.operator == msg.sender
     ensures this.state == IDLE
-    ensures this.operator == sender
+    ensures this.pot == 0
     ensures this.bet == 0
-    ensures this.balance == 0
+    // ensures this != this.operator
+    // ensures this != player
   {
-    this.operator := sender;
-    this.guess := guess;
+    this.operator := msg.sender;
     this.state := IDLE;
-    this.balance := 0;
+    this.pot := 0;
     this.bet := 0;
-    this.player := new Sender();
-    this.isContract := true;
-
+    this.player := new UserAccount(0);
   }
 
-  method removeFrombalance(sender: Sender, amount: int)
+  method addToPot(msg: Msg)
+    requires msg.sender == this.operator
+    requires 0 < msg.value <= msg.sender.balance
     modifies this, this.operator
-    requires this.operator.balance >= 0
-    requires 0 < amount <= this.balance
-    requires this.state != BET_PLACED
-    requires this.operator == sender
-    requires this.operator != this.player
-    ensures this.operator != this.player
-    ensures old(this.player) == this.player
-    ensures this.operator == sender
-    ensures old(this.bet) == this.bet
-    ensures this.operator.balance == old(this.operator.balance) + amount
-    // requires 0 < this.bet < this.balance / 2
+    ensures this.pot == old(this.pot) + msg.value
+    ensures this.operator.balance == old(this.operator.balance) - msg.value
   {
-    this.operator.balance := this.operator.balance + amount;
-    this.balance := balance - amount;
+    this.operator.balance := this.operator.balance - msg.value;
+    this.pot := this.pot + msg.value;
   }
 
+  method removeFromPot(msg: Msg, amount: int)
+    requires this.state != BET_PLACED
+    requires msg.sender == this.operator
+    requires 0 < amount <= this.pot
+    modifies this, this.operator
+    // ensures this.pot == old(this.pot) - amount
+    // ensures this.operator.balance == old(this.operator.balance) + amount
+  {
+    // this.transfer(this.operator,amount);
+    this.pot := this.pot - amount;
+  }
 
-  method createGame(sender: Sender, hashedNumber: int)
+  method createGame(msg: Msg, hashedNumber: int)
     requires this.state == IDLE
-    requires this.operator == sender
-    requires this.player != this.operator
-    requires operator.balance > 0
-    requires this.bet == 0
-    requires this.balance == 0
+    requires msg.sender == this.operator
     modifies this
     ensures this.state == GAME_AVAILABLE
-    ensures this.operator.balance > 0
-    ensures this.player != this.operator
-    ensures this.operator == old(this.operator)
     ensures this.hashedNumber == hashedNumber
-    ensures this.bet == 0
-    ensures this.balance == 0
   {
     this.hashedNumber := hashedNumber;
     this.state := GAME_AVAILABLE;
   }
 
-  method addTobalance(sender: Sender, amount: int)
-    requires 0 < amount <= sender.balance
-    requires sender == this.operator
-    modifies this, this.operator
-    ensures sender.balance == operator.balance
-    ensures old(this.state) == this.state
-    ensures this.operator == old(this.operator)
-    ensures old(this.player) == this.player
-    ensures this.operator.balance >= 0
-    ensures this.hashedNumber == old(this.hashedNumber)
-    ensures this.balance == old(this.balance) + amount
-    ensures this.bet == old(this.bet)
-    // ensures this.operator != this.player
-    // ensures this.operator.balance - amount >= 0
-  {
-    this.operator.balance := this.operator.balance - amount;
-    this.balance := this.balance + amount;
-  }
-
-  method placeBet(sender: Sender, guess : Coin, amount: int)
-    requires state == GAME_AVAILABLE
-    requires sender != this.operator
-    requires 0 < amount <= sender.balance
-    requires this.operator.balance >= 0
-    requires this.balance >= 2 * amount
-
-
-    modifies this, sender, this.operator
-    // ensures 0 < this.bet <= sender.balance
+  method placeBet(msg: Msg, guess: Coin)
+    requires this.state == GAME_AVAILABLE
+    requires msg.sender != this.operator
+    requires 0 < msg.value <= this.pot
+    // requires 0 < msg.value <= msg.sender.balance
+    modifies this, msg.sender
     ensures this.state == BET_PLACED
-    ensures this.operator == old(this.operator)
-    ensures this.bet > 0
-    ensures this.player == sender
-    ensures this.player.balance >= 0
-    ensures this.operator.balance >= 0
-    ensures this.hashedNumber == old(this.hashedNumber)
-    ensures this.balance >= 2 * this.bet
-    // ensures this.operator != this.player
+    ensures this.bet == msg.value
+    ensures this.player == msg.sender
+    ensures this.guess == guess
   {
-
     this.state := BET_PLACED;
-    this.player := sender;
-    sender.transfer(this.operator, amount);
-
-    this.addTobalance(this.operator, amount);
-
-    this.bet := amount;
+    this.player := msg.sender;
+    this.bet := msg.value;
     this.guess := guess;
+
+    //payable ???
+    this.player.balance := this.player.balance - msg.value;
+    this.pot := this.pot + msg.value;
   }
 
-  method decideBet(sender: Sender, secretNumber: int)
+  method decideBet(msg: Msg, secretNumber: int)
     requires this.state == BET_PLACED
-    requires this.operator == sender
-    requires this.bet > 0
-    // requires 0 < this.bet && 0 < operator.balance
-    requires this.player != this.operator
-    // requires this.bet <= this.player.balance
-    requires this.operator.balance >= 0
-    requires this.player.balance >= 0
-    requires this.balance >= 2 * this.bet
+    requires msg.sender == this.operator
+    requires cryptohash(secretNumber) == this.hashedNumber
     modifies this, this.operator, this.player
-
+    ensures this.state == IDLE
+    ensures this.bet == 0
   {
-    var secret: Coin := getCoinFromGuess((secretNumber % 2) == 0);
+    var secret: Coin := getCoinFromNumber(secretNumber);
+
     if secret == this.guess {
       // Player wins
-      this.state := TRANSFERING;
-      this.removeFrombalance(this.operator, 2* this.bet);
-      this.operator.transfer(this.player, 2 * this.bet);
+      this.pot := this.pot - this.bet;
+      // this.transfer(this.player, 2 * this.bet);
+    } else {
+      // Operator wins
+      this.pot := this.pot + this.bet;
     }
     this.bet := 0;
     this.state := IDLE;
   }
-
-}
-
-method Main()
-{
-  var operator := new Sender.FromNameBalance("Operator", 100);
-  var player := new Sender.FromNameBalance("Player", 50);
-
-  var contract := new Contract(operator, HEADS);
-
-  var secretNumber := 42;
-
-  var hashedNumber := contract.cryptohash(secretNumber);
-  contract.createGame(contract.operator, hashedNumber);
-
-  contract.addTobalance(contract.operator,50);
-
-  contract.placeBet(player, TAILS, 10);
-
-  contract.decideBet(contract.operator, 41);
-
-  print "Operator balance: "; print contract.operator.balance; print "\n";
-  print "Player balance: "; print player.balance; print "\n";
-  print "Contract state: "; print contract.state; print "\n";
-  print "balance: "; print contract.balance; print "\n";
-
 }
